\begin{align*}
&\mathbb{Z}_{11} \\
(t,n) &= (3,4)
\end{align*}

\begin{align*}
(x_1, y_1) &= (1,8) \\
(x_2, y_2) &= (4,8) \\
(x_3, y_3) &= (6,5)
\end{align*}

\[
I = \{1,2,3\}.
\]
\begin{align}
s = \sum_{i=1}^{3} y_i\, \prod_{\substack{j \in I \\ j\neq i}} x_j\,(x_j - x_i)^{-1}
\end{align}

Mit den Werten f√ºr $x_i$ und $y_i$ von oben:

\begin{alignat*}{3}
s &= &&\phantom{+} &&8\cdot(4\cdot(4-1)^{-1}\cdot6\cdot(6-1)^{-1}) \\
& &&+ &&8\cdot(1\cdot(1-4)^{-1}\cdot6\cdot(6-4)^{-1}) \\
& &&+ &&5\cdot(1\cdot(1-6)^{-1}\cdot4\cdot(4-6)^{-1}) \\
&= &&\phantom{+} &&8\cdot(4\cdot3^{-1}\cdot6\cdot5^{-1}) \\
& &&+ &&8\cdot(1\cdot(-3)^{-1}\cdot6\cdot2^{-1}) \\
& &&+ &&5\cdot(1\cdot(-5)^{-1}\cdot4\cdot(-2)^{-1}) \\
&\equiv &&\phantom{+} &&(-1)\cdot6\cdot4^{-1} + 4\cdot(-6)^{-1} + (-2)\cdot(-1)^{-1} \\
&\equiv &&- &&7 + 3 + 2 \\
&\equiv && &&9
\end{alignat*}
